proofs/isabelle/SpecRest/core/Translate.thy
@@ -36,6 +36,7 @@ fun translate :: "expr \<Rightarrow> smt_term" where
 | "translate (ForallRel var rel_n body _)  = TForallRel  var rel_n (translate body)"
 | "translate (ForallSet var setE body _)   = TForallSet  var (translate setE) (translate body)"
 | "translate (TheRel var rel_n body _)     = TTheRel     var rel_n (translate body)"
+| "translate (EntityBase name _)           = TEntityBase name"
 | "translate (Prime e _) = TPrime (translate e)"
 | "translate (Pre e _)   = TPre   (translate e)"
 | "translate (CardRel rel_name _)          = TCardRel rel_name"
